Question 1: $$
\begin{align}
\text{At }x=0&:K=-\Delta U=\frac{1}{2}kx_{0}^{2} \\
\text{Friction } f \text{ at }x=d&:-\left( \mu_{0}mg+\mu_{1}\frac{d}{d}mg \right) \\
\Delta K \text{ between }x=0 \text{ and } x=d&:-(\mu_{0}mgd+\mu_{1}mgd) \\
\text{At }x=d&:K=\frac{1}{2}kx_{0}^{2}-(\mu_{0}mgd+\mu_{1}mgd) \\
\text{At }h&:K=mgh \\
\implies h&=\frac{1}{2}kx_0^2-\mu_{0}d-\mu_{1}d
\end{align}
$$
Question 2:
(a) 90Ëš
(b) $$
\begin{align}
mgR&=\frac{1}{2}mv^{2} \\
2gR&=v^{2} \\
\therefore v&=\sqrt{2gR}
\end{align}
$$
Question 3:
$$
\begin{align}
\text{At the top of the hoop}:kd=mg \implies k=\frac{mg}{d}
\end{align}
$$
Question 4:
(a)
$$
\begin{align}
\text{After collision:} \\
(m_{1}+m_{2})v&=m_{1}v_{1} \\
v&=\frac{m_{1}v_{1}}{m_{1}+m_{2}} \\
\text{Kinetic energy:} \\
K&=\frac{1}{2}mv^{2}=\frac{1}{2}(m_{1}+m_{2})\left(\frac{m_{1}v_{1}}{m_{1}+m_{2}}\right)^{2} \\
&=\frac{(m_{1}v_{1})^{2}}{2(m_{1}+m_{2})} \\
\text{Potential energy at max height}&=mgh \\
(m_{1}+m_{2})gh&=\frac{(m_{1}v_{1})^{2}}{2(m_{1}+m_{2})} \\
\therefore h&=\frac{(m_{1}v_{1})^{2}}{2g}
\end{align}
$$
(b)
$$
\begin{align}
E_{f}&=\frac{(m_{1}v_{1})^{2}}{2(m_{1}+m_{2})} \\
E_{i}&=\frac{m_{1}v_{1}}{2} \\
\therefore \frac{E_{f}}{E_{i}}&=\frac{\frac{(m_{1}v_{1})^{2}}{2(m_{1}+m_{2})}}{\frac{m_{1}v_{1}}{2}} \\
&=\frac{m_{1}v_{1}}{m_{1}+m_{2}}
\end{align}
$$
Question 5:
Let rightwards be positive for this question.
(a)
$$
\begin{align}
m_Av_0 &= m_Bv_B-m_Av_A \\
v_A&=\frac{m_Bv_B}{m_A}-v_0 \implies v_A^2=\frac{m_B^2v_B^2}{m_A^2}-2\frac{m_Bv_B}{m_A}v_0+v_0^2 \\
v_B&=\frac{m_A}{m_B}(v_0-v_A) \implies v_B^2=\frac{m_A^2}{m_B^2}(v_0^2-2v_0v_A+v_A^2) \\\\
\text{Since the collision is elastic,} \\
\frac{1}{2}m_Av_0^2&=\frac{1}{2}m_Av_A^2+\frac{1}{2}m_Bv_B^2 \\
\implies m_Av_0^2&=m_Av_A^2+m_Bv_B^2 \\
v_A^2&=v_0^2-\frac{m_Bv_B^2}{m_A} \\
v_B^2&=\frac{m_A}{m_B}(v_0^2-v_A^2) \\
 \\
\frac{m_B^2v_B^2}{m_A^2}-2\frac{m_Bv_B}{m_A}v_0+v_0^2 &= v_0^2-\frac{m_Bv_B^2}{m_A} \\
2v_0-v_B\frac{m_B}{m_A} &=v_B \\
v_B\frac{m_B}{m_A}+v_B &=2v_0 \\
v_B\left( \frac{m_B}{m_A}+1 \right) &=2v_0 \\
\therefore v_B &=\frac{2v_0m_A}{m_B+m_A} \\
 \\
\frac{m_A}{m_B}(v_0^2-v_A^2)&=\frac{m_A^2}{m_B^2}(v_0^2-2v_0v_A+v_A^2) \\
(v_0^2-v_A^2)&=\frac{m_A}{m_B}(v_0^2-2v_0v_A+v_A^2)
\end{align}
$$
(b)
$$
\begin{align}
v_{B}-0&=\frac{v_{B}}{2}-v'_{B} \\
\therefore v'_{B}&=-\frac{v_{B}}{2}
\end{align}
$$
(c)
$$
\begin{align}

\end{align}
$$